theories/iris/examples/stack/function/new_stack.v
@@ -47,6 +47,8 @@ End code.
 
 Section specs.
 
+
+  
   Definition overflow : N -> Prop :=
     λ len, (Wasm_int.Int32.modulus - 1)%Z <> Wasm_int.Int32.Z_mod_modulus (ssrnat.nat_of_bin (len `div` page_size)).
 
